LL1/ParseTableLemmas.v
@@ -1,0 +1,42 @@
+Require Import ExampleGrammars.
+Require Import Grammar.
+Require Import Lemmas.
+Require Import List MSets String.
+Require Import ExampleGrammars Grammar Lemmas
+               Tactics ParseTable Utils.
+Import ListNotations.
+Open Scope list_scope.
+
+Lemma nullable_nonrec :
+  forall g sym,
+    (@nullable_sym g) sym
+    -> exists gamma,
+      (@nullable_prod g) sym gamma
+      /\ ~In sym gamma.
+Proof.
+  intros g sym.
+  induction 1 using nullable_sym_mutual_ind with
+      (P := fun sym gamma (pf : nullable_prod sym gamma) =>
+              exists gamma',
+                (@nullable_prod g) sym gamma'
+                /\ ~In sym gamma')
+      (P0 := fun gamma (pf : nullable_gamma gamma) =>
+               forall sym,
+                 In sym gamma
+                 -> exists gamma',
+                   nullable_prod sym gamma'
+                   /\ ~In sym gamma')
+      (P1 := fun sym (pf : nullable_sym sym) =>
+               exists gamma,
+                 (@nullable_prod g) sym gamma
+                 /\ ~In sym gamma); intros.
+  - destruct (List.In_dec symbol_eq_dec (NT x) ys).
+    + apply IHnullable_sym in i0.
+      eauto.
+    + exists ys.
+      split; auto.
+      constructor; auto.
+  - inv H.
+  - inv H0; eauto.
+  - eauto.
+Qed.
